---
title: "Gumbel Regression"
output: rmarkdown::html_vignette
vignette: >
  %\VignetteIndexEntry{Gumbel Regression}
  %\VignetteEngine{knitr::rmarkdown}
  \usepackage[utf8]{inputenc}
---

The CDF of Gumbel Distribution with location parameter $mu$ and scale parameter $\sigma$ is:

$$F(x | \mu, \sigma) = \frac{1}{\sigma} e^{-(z + e^{-z})}$$

where $z = \frac{x - \mu}{\sigma}$.

In addition, we set $s = log(\sigma)$ so that $s \in \mathbb{R}$.

The implemented Gumbel Regression is:

$$y \approx Gumbel(\mu = x_i^T \beta, \sigma = e^s)$$

Therefore, the loss function which is the average of the negative log likelihood function:

$$\begin{eqnarray}
L(s, \beta) &=& \frac{1}{n}\sum_{i=1}^n{z_i + e^{-z_i} + s} \\
&=& s + \frac{1}{n}\sum_{i=1}^n{z_i + e^{-z_i}} \\
&=& s + \frac{1}{n}\sum_{i=1}^n L'(z_i)
\end{eqnarray}$$

where:

- $n$ is the sample size
- $z_i = \frac{y_i - x_i^T \beta}{e^s}$

In the returned function from `get.loss`, `get.gradient` and `get.Hv`,
there is a parameter `w` which is $(s, \beta)$.

## Helper Derivatives

$$\begin{eqnarray}
\frac{\partial}{\partial s}z_i = -z_i
\end{eqnarray}$$

$$\begin{eqnarray}
\frac{\partial}{\partial \beta}z_i = - \frac{x_i}{e^s}
\end{eqnarray}$$

$$\begin{eqnarray}
\frac{\partial}{\partial z_i}L'(z_i) = 1 - e^{-z_i}
\end{eqnarray}$$

## Gradient

$$\begin{eqnarray}
\frac{\partial}{\partial s}L &=& 1 + \frac{1}{n}\sum_{i=1}^n {\frac{\partial L'(z_i)}{\partial z_i} \times \frac{\partial z_i}{\partial s}} \\ 
&=& 1 + \frac{1}{n}\sum_{i=1}^n{(1 - e^{-z_i}) \times (-z_i)} \\
&=& 1 + \frac{1}{n}\sum_{i=1}^n{z_i e^{-z_i} - z_i}
\end{eqnarray}$$

$$\begin{eqnarray}
\frac{\partial}{\partial \beta}L &=& \frac{1}{n}\sum_{i=1}^n {\frac{\partial L'(z_i)}{\partial z_i} \times \frac{\partial z_i}{\partial \beta}} \\ 
&=& \frac{1}{n}\sum_{i=1}^n {(1 - e^{-z_i}) \times \frac{-x_i}{e^s}} \\
&=& \frac{1}{n}\sum_{i=1}^n {\frac{e^{-z_i} - 1}{e^s} x_i}
\end{eqnarray}$$

## Hessian

$$\begin{eqnarray}
\frac{\partial^2}{\partial s^2}L &=& \frac{1}{n}\sum_{i=1}^n{\frac{\partial}{\partial s}(z_i e^{-z_i} - z_i)} \\
&=& \frac{1}{n}\sum_{i=1}^n{ z_i^2 e^{-z_i} - z_i e^{-z_i} + z_i}
\end{eqnarray}$$

$$\begin{eqnarray}
\frac{\partial^2}{\partial s \partial \beta}L &=& \frac{1}{n}\sum_{i=1}^n{\frac{\partial}{\partial \beta}(z_i e^{-z_i} - z_i)} \\
&=& \frac{1}{n}\sum_{i=1}^n {\frac{z_i e^{-z_i} - e^{-z_i} +1}{e^s} x_i}
\end{eqnarray}$$

$$\begin{eqnarray}
\frac{\partial^2}{\partial \beta^2}L &=& \frac{1}{n}\sum_{i=1}^n{\frac{\partial}{\partial \beta}(\frac{e^{-z_i} - 1}{e^s} x_i)} \\
&=& \frac{1}{n}\sum_{i=1}^n {\frac{e^{-z_i}}{e^{2s}} x_i x_i^T}
\end{eqnarray}$$
